src/dafny/refinement/evmir-refinement-general.dfy
@@ -50,73 +50,302 @@ module EVMIRSimulationFull {
                     EVMProg2.Jump(2),               // 2
                     EVMProg2.AInst(b2)              // 3
                 ]
-            case _ =>   //  Cases not covered
-                []
+            case While(c, xb) => 
+                //   Translate xb into EVM. xbb goes from 0 to |xbb| - 1
+                var xbb := toEVM(xb);
+                //  transaliton of While is 0 -> jumpi, 1..|xbb| xbb, xbb + 1 -> Jump
+                [EVMProg2.Jumpi(negF(c), |xbb| + 2)] + xbb + [ EVMProg2.Jump(-(|xbb| + 1))]
+            case IfElse(cond, xb1, xb2) => 
+                var xbb1 := toEVM(xb1);
+                var xbb2 := toEVM(xb2);
+                [EVMProg2.Jumpi(negF(cond), |xbb1| + 1)] + 
+                    xbb1 + 
+                [ EVMProg2.Jump(|xbb2| + 1)] +
+                    xbb2
+
+                // [
+                //     EVMProg2.Jumpi(negF(cond), 3),  // 0
+                //     EVMProg2.AInst(b1),             // 1
+                //     EVMProg2.Jump(2),               // 2
+                //     EVMProg2.AInst(b2)              // 3
+                // ]
+            // case _ => //  Cases not covered
+            //     []
     }
 
+    /**
+     *  Jumps in the EVM programs are within [0, |toEVM(p)|].
+     */
+    lemma foo202(p: EVMIRProg) 
+        ensures isBounded(toEVM(p))
+    {
+        match p 
+            case Block(i) => 
+            case While(c, Block(b)) => 
+            case IfElse(cond, Block(b1), Block(b2)) => 
+            case While(c, xb) => 
+                var xbb := toEVM(xb);
+                var whileEVM :=  [EVMProg2.Jumpi(negF(c), |xbb| + 2)] + xbb + [ EVMProg2.Jump(-(|xbb| + 1))];
+                assert toEVM(While(c, xb)) == whileEVM;
+                forall (i: nat | 0 <= i < |whileEVM|) 
+                    ensures boundedIns(whileEVM, i)
+                {
+                    if 1 <= i < |whileEVM| - 1 {
+                        //  Instruction i in whileEVM is intruction i - 1 xbb 
+                        foo202(xb); 
+                        match whileEVM[i] 
+                            case Jumpi(cond, tgt) => 
+                                //  Jump must be to an instruction between 1 and |whileEVM| - 1
+                                calc ==> {
+                                    //  Induction on xbb
+                                    boundedIns(xbb, i - 1);
+                                    0 <= i - 1 + tgt <= |xbb|;
+                                    calc == {
+                                        |xbb|;
+                                        |whileEVM| - 2;  
+                                    }
+                                    0 <= i - 1 + tgt <= |whileEVM| - 2;
+                                    1 <= i + tgt <= |whileEVM| - 1;
+                                    0 <= i + tgt <= |whileEVM|;
+                                }
+                            case Jump(tgt) => 
+                                //  Jump must be to an instruction between 1 and |whileEVM| - 1
+                                calc ==> {
+                                    boundedIns(xbb, i - 1);
+                                    0 <= i - 1 + tgt <= |xbb|;
+                                    calc == {
+                                        |xbb|;
+                                        |whileEVM| - 2;   
+                                    }
+                                    0 <= i - 1 + tgt <= |whileEVM| - 2;
+                                    1 <= i + tgt <= |whileEVM| - 1;
+                                    0 <= i + tgt <= |whileEVM|;
+                                }
+                            case _ => 
+                    } else {
+                        //  i == 0 or i == |whileEVM| - 1
+                        assert boundedIns(whileEVM, 0);
+                        assert boundedIns(whileEVM, |whileEVM| - 1);
+                    }
+                }
+            case IfElse(cond, xb1, xb2) => 
+                var xbb1 := toEVM(xb1);
+                var xbb2 := toEVM(xb2);
+                var ifElseEVM := [EVMProg2.Jumpi(negF(cond), |xbb1| + 1)] + 
+                    xbb1 +                      //  instructions from 1 to |xbb1|
+                [ EVMProg2.Jump(|xbb2| + 1)] +  //  instruction |xbb1| + 1
+                    xbb2;                       //  instructions from |xbb1| + 2 to |xbb1| + 2 + |xbb2|
+                assert toEVM(IfElse(cond, xb1, xb2)) == ifElseEVM;
+                forall (i: nat | 0 <= i < |ifElseEVM|) 
+                    ensures boundedIns(ifElseEVM, i)
+                {
+                    if 1 <= i <= |xbb1| {
+                        foo202(xb1);
+                        //  ifElseEVM[i] is xbb[i - 1]
+                        match ifElseEVM[i]
+                            case Jumpi(cond, tgt) => 
+                                 calc ==> {
+                                    boundedIns(xbb1, i - 1);
+                                    0 <= i - 1 + tgt <= |xbb1|;
+                                    1 <= i + tgt <= |xbb1| + 1;
+                                    calc <= {
+                                        |xbb1| + 1;
+                                        |ifElseEVM|;  
+                                    }
+                                    0 <= i + tgt <= |ifElseEVM|; 
+                                }
+                            case Jump(tgt) => 
+                                calc ==> {
+                                    boundedIns(xbb1, i - 1);
+                                    0 <= i - 1 + tgt <= |xbb1|;
+                                    1 <= i + tgt <= |xbb1| + 1;
+                                    calc <= {
+                                        |xbb1| + 1;
+                                        |ifElseEVM|;  
+                                    }
+                                    0 <= i + tgt <= |ifElseEVM|; 
+                                }
+                            case _ => 
+                    } else if |xbb1| + 2 <= i < |ifElseEVM| {
+                        foo202(xb2);
+                        //  ifElseEVM[i] is xbb2[i - (|xbb1| + 2)]
+                        match ifElseEVM[i]
+                            case Jumpi(cond, tgt) => 
+                                 calc ==> {
+                                    boundedIns(xbb2, i - (|xbb1| + 2));
+                                    0 <= i - (|xbb1| + 2) + tgt <= |xbb2|;
+                                    |xbb1| + 2 <= i + tgt <=  |xbb2| + (|xbb1| + 2);
+                                    calc <= {
+                                        |xbb2| + (|xbb1| + 2);
+                                        |ifElseEVM|;  
+                                    }
+                                    0 <= i + tgt <= |ifElseEVM|; 
+                                }
+                            case Jump(tgt) => 
+                                calc ==> {
+                                    boundedIns(xbb2, i - (|xbb1| + 2));
+                                    0 <= i - (|xbb1| + 2) + tgt <= |xbb2|;
+                                    |xbb1| + 2 <= i + tgt <=  |xbb2| + (|xbb1| + 2);
+                                    calc <= {
+                                        |xbb2| + (|xbb1| + 2);
+                                        |ifElseEVM|;  
+                                    }
+                                    0 <= i + tgt <= |ifElseEVM|; 
+                                }
+                            case _ => 
+                    } else {
+                        assert i == 0 || i == |xbb1| + 1;
+                        assert boundedIns(ifElseEVM, i);
+                    } 
+                }
+    }
+
+    // lemma foo303()
+
+    /**
+     *  Single While loop. Assume Unique block in loop body.
+     *
+     *  @returns    The (minimum) number of steps in the EVMIR to simulate n steps in EVM. 
+     */
+    lemma {:verify false} foo101<S>(xb: EVMIRProg, n: nat, s: S) returns (k: nat)
+        // requires n > 1
+        // requires n < 3
+        ensures k <= n && runEVMIR2([xb], s, k).0 == runEVM2(0, toEVM(xb), s, n).0
+    {
+        if n < 1 {
+            k := 0;
+        } else {
+            match xb 
+                case Block(i) => 
+                    calc == {
+                        runEVM2(0, toEVM(xb), s, n).0;
+                        runEVM2(0, [EVMProg2.AInst(i)], s, n).0;
+                        runInst(i, s);
+                        runEVMIR2([Block(i)], s, n).0;
+                        runEVMIR2([xb], s, n).0;
+                    }
+                    k := n ;
+                case While(c, xb) => 
+                    var xbb := toEVM(xb);
+                    var whileEVM :=  [EVMProg2.Jumpi(negF(c), |xbb| + 2)] + xbb + [ EVMProg2.Jump(-(|xbb| + 2))];
+                    if c(s) {
+                        if n == 1 {
+                            k := n;
+                        } else {
+                            assert n >= 2;
+                            //  do one step in toEVM(While(c, xb))
+                            //  target state is s1 
+                            calc == {
+                                runEVM2(0, whileEVM, s, n);
+                                runEVM2(1, whileEVM, s, n - 1);
+                                // (s, |xbb| + 2);
+                            }  
+                            var (s', n') := runEVMIR2([xb], s, n - 1);
+                            //  From s1, run toEVM(xb). Match with k1 steps in xb
+
+                            //  first n steps of toEVM(While(c, xb)) can be simulated by 
+                            //  1 + k1 
+
+                            //  Then finish running
+
+                            //  Use n - 1 steps to simulate toEVM(xb) 
+                            var (s1, n1) := runEVM2(0, toEVM(xb), s, n - 1);       
+                            if n1 < 2 {
+                                k := 0;
+                            } else {
+                                k := 1;
+                            }
+                            // calc == {
+
+                            // }
+                            k := 0;
+                            assume runEVMIR2([While(c, xb)], s, k).0 == runEVM2(0, toEVM(While(c, xb)), s, n).0;
+                        }
+                    } else {
+                        //  Condition is false, exit the loop and the jump program
+                        assert negF(c)(s);
+                        calc == {
+                            runEVM2(0, whileEVM, s, n);
+                            runEVM2(|xbb| + 2, whileEVM, s, n - 1);
+                            (s, |xbb| + 2);
+                        }  
+                        //  In the while program, same state is reached in 1 step.
+                        calc == {
+                            runEVMIR2([While(c, xb)], s, n);
+                            runEVMIR2([While(c, xb)][1..], s , n - 1);
+                            (s, n - 1);
+                        }
+                        k := n;
+                    }
+                case IfElse(c, xb1, xb2)=> 
+                    k := 0;
+                    assume runEVMIR2([IfElse(c, xb1, xb2)], s, k).0 == runEVM2(0, toEVM(IfElse(c, xb1, xb2)), s, n).0;
+        }
+    }
+        
     //  Translation proof (simple)
     /**
      *  Single While loop. Assume Unique block in loop body.
      *
      *  @returns    The (minimum) number of steps in the EVMIR to simulate n steps in EVM. 
      */
-    // lemma singleWhileSim<S>(i: EVMInst, cond: S -> bool, n: nat, s: S) returns (k: nat)
-    //      ensures k <= n && runEVMIR([While(cond, Block(i))], s, k) ==
-    //         runEVM(
-    //             1,
-    //             toEVM(While(cond, Block(i))),
-    //             s, 
-    //             n).0
-    // {
-    //     //  For convenience and clarity, store program in a var 
-    //     var p :=  toEVM(While(cond, Block(i)));
-    //     if n < 2 {
-    //         //  Only one step can be simulated so the instruction at pc is not executed.
-    //         k := 0;
-    //     } else if n < 3 {
-    //         //  Exactly two steps in the EVM. 
-    //         assert n == 2;
-    //         if cond(s) {
-    //             k := 1;
-    //         } else {
-    //             assert !cond(s);
-    //             k := 0;
-    //         }
-    //     } else {
-    //         //  More than 2 steps in the EVM. So at least one iteration of the EVM body.
-    //         assert n > 2;
-    //         if cond(s) {
-    //             calc == {
-    //                 runEVM(1, p, s, n);
-    //                 runEVM(2, p, s, n - 1);
-    //                 runEVM(3, p, runInst(i, s), n - 2);
-    //                 runEVM(1, p, runInst(i, s), n - 3);
-    //             }
-    //             //  Because body of while and jump progs are the same, they reach the same
-    //             //  state after one iteration of the body.
-    //             calc == {
-    //                 runEVMIR([While(cond, Block(i))], s, n);
-    //                 runEVMIR([While(cond, Block(i))], runInst(i, s), n - 1);
-    //             }
-    //             //  And by induction, we can get a simulation for the n - 3 remaining steps compute the same
-    //             //  result.
-    //             var xk := singleWhileSim(i, cond, n - 3, runInst(i, s));
-    //             //  Overall we do the body of the loop once and then in xk steps simulate the rest.
-    //             k := 1 + xk;
-    //         } else {
-    //             //  Exit the loop.
-    //             assert !cond(s);
-    //             k := 1;
-    //         }    
-    //     }
-    // }    
+    lemma {:verify false} singleWhileSim<S>(i: EVMInst, cond: S -> bool, n: nat, s: S) returns (k: nat)
+         ensures k <= n && runEVMIR([While(cond, Block(i))], s, k) ==
+            runEVM2(
+                0,
+                toEVM(While(cond, Block(i))),
+                s, 
+                n).0
+    {
+        //  For convenience and clarity, store program in a var 
+        var p :=  toEVM(While(cond, Block(i)));
+        if n < 2 {
+            //  Only one step can be simulated so the instruction at pc is not executed.
+            k := 0;
+        } else if n < 3 {
+            //  Exactly two steps in the EVM. 
+            assert n == 2;
+            if cond(s) {
+                k := 1;
+            } else {
+                assert !cond(s);
+                k := 0;
+            }
+        } else {
+            //  More than 2 steps in the EVM. So at least one iteration of the EVM body.
+            assert n > 2;
+            if cond(s) {
+                calc == {
+                    runEVM2(0, p, s, n);
+                    runEVM2(1, p, s, n - 1);
+                    runEVM2(2, p, runInst(i, s), n - 2);
+                    runEVM2(0, p, runInst(i, s), n - 3);
+                }
+                //  Because body of while and jump progs are the same, they reach the same
+                //  state after one iteration of the body.
+                calc == {
+                    runEVMIR([While(cond, Block(i))], s, n);
+                    runEVMIR([While(cond, Block(i))], runInst(i, s), n - 1);
+                }
+                //  And by induction, we can get a simulation for the n - 3 remaining steps compute the same
+                //  result.
+                var xk := singleWhileSim(i, cond, n - 3, runInst(i, s));
+                //  Overall we do the body of the loop once and then in xk steps simulate the rest.
+                k := 1 + xk;
+            } else {
+                //  Exit the loop.
+                assert !cond(s);
+                k := 1;
+            }    
+        }
+    }    
         
     /**
      *  If Then Else Simulation proof. Assume unique block in ifBody and ifElse.
      *
      *  @returns    The (minimum) number of steps in the EVMIR to simulate n steps in EVM. 
      */
-    lemma ifTheElseSim<S>(i1: EVMInst, i2: EVMInst, cond: S -> bool, n: nat, s: S) returns (k: nat)
+    lemma {:verify false} ifTheElseSim<S>(i1: EVMInst, i2: EVMInst, cond: S -> bool, n: nat, s: S) returns (k: nat)
         requires n > 2
         ensures k <= n && runEVMIR([IfElse(cond, Block(i1), Block(i2))], s, k) ==  
             runEVM2(
